src/Std/Data/Iterators/Combinators/Monadic/DropWhile.lean
@@ -286,4 +286,12 @@ instance DropWhile.instIteratorForPartial [Monad m] [Monad n] [Iterator α m β]
     IteratorLoopPartial (DropWhile α m β P) m n :=
   .defaultImplementation
 
+instance {α : Type w} [Monad m] [Iterator α m β] [Finite α m] [IteratorLoop α m m] {P} :
+    IteratorSize (DropWhile α m β P) m :=
+  .defaultImplementation
+
+instance {α : Type w} [Monad m] [Iterator α m β] [IteratorLoopPartial α m m] {P} :
+    IteratorSizePartial (DropWhile α m β P) m :=
+  .defaultImplementation
+
 end Std.Iterators
