src/Std/Data/Iterators/Combinators/Monadic/Take.lean
@@ -148,4 +148,12 @@ instance Take.instIteratorLoopPartial [Monad m] [Monad n] [Iterator α m β]
     IteratorLoopPartial (Take α m β) m n :=
   .defaultImplementation
 
+instance {α : Type w} [Monad m] [Iterator α m β] [Finite α m] [IteratorLoop α m m] :
+    IteratorSize (Take α m β) m :=
+  .defaultImplementation
+
+instance {α : Type w} [Monad m] [Iterator α m β] [IteratorLoopPartial α m m] :
+    IteratorSizePartial (Take α m β) m :=
+  .defaultImplementation
+
 end Std.Iterators
